%%% Ne pas modifier jusqu'à la ligne 25
\documentclass[a4paper,12pt]{book}
\usepackage[utf8]{inputenc}
\usepackage[french]{babel}
%%\usepackage{CJK}
\usepackage{yhmath}
\usepackage[left=2cm,right=2cm,top=3cm,bottom=2cm, headheight=1.5cm,headsep=1.5cm]{geometry}
%%\usepackage{CJKutf8}
\usepackage{amsfonts}
\usepackage{mathrsfs}
\usepackage{amsmath,amsfonts,amssymb,dsfont}
\usepackage{graphicx}
\usepackage{subfigure}
\usepackage{enumitem}		%\enumerate-resume
\usepackage[colorlinks=true,unicode={true},hyperindex=false, linkcolor=blue, urlcolor=blue]{hyperref}
\newcommand{\myref}[1]{\ref{#1} page \pageref{#1}}

\addto\captionsfrench{\def\tablename{Tableau}}  %légendes des tableaux
\renewcommand\thesection{\Roman{section}~-~} 
\renewcommand\thesubsection{\Roman{section}.\Alph{subsection}~-~} 
\renewcommand\thesubsubsection{\Roman{section}.\Alph{subsection}.\arabic{subsubsection}~-~} 

\newcommand{\conclusion}[1]{\newline \centerline{\fbox{#1}}}

\setcounter{secnumdepth}{3}
\parindent=0pt

\usepackage{fancyhdr}
\pagestyle{fancy}

\lhead{SJTU-ParisTech} 
%%%%%%%%%%%%%%%%%%%%%%%%%%%%%%%%%%
\chead{DM5}
\rhead{Daniel 518261910024}

\begin{document}
\renewcommand{\labelitemi}{$\blacktriangleright$}
\renewcommand{\labelitemii}{$\bullet$}



\section{}
\begin{itemize}
    \item 1.a $\mathbb{N}^{*}$
    \item 1.b $\mathbb{P}(X \geq x)=(1-p)^{x-1}$
    \item 1.c $\mathbb{P}(T \geq t)=\mathbb{P}(X \geq t)\mathbb{P}(Y \geq t)=(1-p)^{2t-2}$
    \item 1.d $\mathbb{P}(T=t)= (1-p)^{2t-2}(2p-p^2)$
\end{itemize}
\section{}
\begin{itemize}
    \item 2.a $\mathbb{N}$
    \item 2.b $\frac{p}{p-1}\ln p$
    \item 2.c 
\end{itemize}


\begin{align*}
    (T=t) &= (X=t,Y>t)\cup(X>t,Y=t)\cup(X=t,Y=t)\\
    &=\bigcup_{i=t+1}^{\infty}(X=t,Y=i)\cup\bigcup_{j=t+1}^{\infty}(X=j,Y=t)\cup(X=t,Y=t)
\end{align*}

\begin{align*}
    \mathbb{P}(T=t)&=\sum_{i=t+1}^{+\infty}\mathbb{P}(X=t,Y=i)+\sum_{j=t+1}^{+\infty}\mathbb{P}(X=j,Y=t)+\mathbb{P}(X=t,Y=t)\\
    &=\sum_{i=t+1}^{+\infty}\mathbb{P}(X=t)\mathbb{P}(Y=i)+\sum_{j=t+1}^{+\infty}\mathbb{P}(X=j)\mathbb{P}(Y=t)+\mathbb{P}(X=t)\mathbb{P}(Y=t)\\
    &=p(1-p)^{t-1}\sum_{i=t+1}^{+\infty}p(1-p)^{i-1}+p(1-p)^{t-1}\sum_{j=t+1}^{+\infty}p(1-p)^{j-1}+p(1-p)^{t-1}*p(1-p)^{t-1}\\
    &=2p(1-p)^{t-1}(1-p)^t+p^2(1-p)^{2t-2}\\
    &=p(2-p)(1-p)^{2t-2}
\end{align*}

\begin{align*}
    (T=t,Z=0)&=(\min(X,Y)=t,X=Y)\\
    \mathbb{P}(T=t,Z=0)&=\mathbb{P}(X=t,Y=t)=\mathbb{P}(X=t)\mathbb{P}(Y=t)\\
    &=p(1-p)^{t-1}*p(1-p)^{t-1}=p(2-p)(1-p)^{2t-2}\\
    &=\left(p(2-p)(1-p)^{2t-2}\right)\left(\frac{p}{2-p}\right)\\
    &=\mathbb{P}(T=t)\mathbb{P}(Z=0)
\end{align*}

\begin{align*}
    (T=t,Z=z)&=(\min(X,Y)=t,|X-Y|=z)=(X=t,Y=z+t)\cup(X=z+t,Y=t)\\
    \mathbb{P}(T=t,Z=z)&=\mathbb{P}(X=t,Y=t+z)+\mathbb{P}(X=t+z,Y=t)\\
    &=\mathbb{P}(X=t)\mathbb{P}(Y=t+z)+\mathbb{P}(X=t+z)\mathbb{P}(Y=t)\\
    &=2p(1-p)^{t-1}*p(1-p)^{t+z-1}\\
    &=\left(p(2-p)(1-p)^{2t-2}\right)\left((1-p)^z\frac{2p}{2-p}\right)\\
    &=\mathbb{P}(T=t)\mathbb{P}(Z=z)    
\end{align*}
$1-p \in ]0,1[$
\end{document}